module plfa.Induction where

import Relation.Binary.PropositionalEquality as Eq
open Eq using (_≡_; refl; cong; sym)
open Eq.≡-Reasoning using (begin_; step-≡-∣; step-≡-⟩; _∎)
open import Data.Nat using (ℕ; zero; suc; _+_; _*_; _∸_; _^_)

+-assoc : ∀ (m n p : ℕ) → (m + n) + p ≡ m + (n + p)
+-assoc zero n p =
    begin
        (zero + n) + p
    ≡⟨⟩
        n + p
    ≡⟨⟩
        zero + (n + p)
    ∎
+-assoc (suc m) n p =
  begin
    (suc m + n) + p
  ≡⟨⟩
    suc (m + n) + p
  ≡⟨⟩
    suc ((m + n) + p)
  ≡⟨ cong suc (+-assoc m n p) ⟩
    suc (m + (n + p))
  ≡⟨⟩
    suc m + (n + p)
  ∎

+-assoc-0 : ∀ (n p : ℕ) → (0 + n) + p ≡ 0 + (n + p)
+-assoc-0 n p =
  begin
    (0 + n) + p
  ≡⟨⟩
    n + p
  ≡⟨⟩
    0 + (n + p)
  ∎

+-assoc-1 : ∀ (n p : ℕ) → (1 + n) + p ≡ 1 + (n + p)
+-assoc-1 n p =
  begin
    (1 + n) + p
  ≡⟨⟩
    suc (0 + n) + p
  ≡⟨⟩
    suc ((0 + n) + p)
  ≡⟨ cong suc (+-assoc-0 n p) ⟩
    suc (0 + (n + p))
  ≡⟨⟩
    1 + (n + p)
  ∎

+-assoc-2 : ∀ (n p : ℕ) → (2 + n) + p ≡ 2 + (n + p)
+-assoc-2 n p =
  begin
    (2 + n) + p
  ≡⟨⟩
    suc (1 + n) + p
  ≡⟨⟩
    suc ((1 + n) + p)
  ≡⟨ cong suc (+-assoc-1 n p) ⟩
    suc (1 + (n + p))
  ≡⟨⟩
    2 + (n + p)
  ∎

+-identityʳ : ∀ (m : ℕ) → m + zero ≡ m
+-identityʳ zero =
  begin
    zero + zero
  ≡⟨⟩
    zero
  ∎
+-identityʳ (suc m) =
  begin
    suc m + zero
  ≡⟨⟩
    suc (m + zero)
  ≡⟨ cong suc (+-identityʳ m) ⟩
    suc m
  ∎

+-suc : ∀ (m n : ℕ) → m + suc n ≡ suc (m + n)
+-suc zero n =
  begin
    zero + suc n
  ≡⟨⟩
    suc n
  ≡⟨⟩
    suc (zero + n)
  ∎
+-suc (suc m) n =
  begin
    suc m + suc n
  ≡⟨⟩
    suc (m + suc n)
  ≡⟨ cong suc (+-suc m n) ⟩
    suc (suc (m + n))
  ≡⟨⟩
    suc (suc m + n)
  ∎

+-comm : ∀ (m n : ℕ) → m + n ≡ n + m
+-comm m zero =
  begin
    m + zero
  ≡⟨ +-identityʳ m ⟩
    m
  ≡⟨⟩
    zero + m
  ∎

+-comm m (suc n) =
  begin
    m + suc n
  ≡⟨ +-suc m n ⟩
    suc (m + n)
  ≡⟨ cong suc (+-comm m n) ⟩
    suc (n + m)
  ≡⟨⟩
    suc n + m
  ∎

+-rearrange : ∀ (m n p q : ℕ) → (m + n) + (p + q) ≡ m + (n + p) + q
+-rearrange m n p q =
  begin
    (m + n) + (p + q)
  ≡⟨ sym (+-assoc (m + n) p q) ⟩
    ((m + n) + p) + q
  ≡⟨ cong (_+ q) (+-assoc m n p) ⟩
    (m + (n + p)) + q
  ∎

+-assoc′ : ∀ (m n p : ℕ) → (m + n) + p ≡ m + (n + p)
+-assoc′ zero n p = refl
+-assoc′ (suc m) n p rewrite +-assoc′ m n p = refl 

+-identity′ : ∀ (n : ℕ) → n + zero ≡ n
+-identity′ zero = refl
+-identity′ (suc n) rewrite +-identity′ n = refl

+-suc′ : ∀ (m n : ℕ) → m + suc n ≡ suc (m + n)
+-suc′ zero n = refl
+-suc′ (suc m) n rewrite +-suc′ m n = refl

+-comm′ : ∀ (m n : ℕ) → m + n ≡ n + m
+-comm′ m zero rewrite +-identity′ m = refl
+-comm′ m (suc n) rewrite +-suc′ m n | +-comm′ m n = refl

+-swap : ∀ (m n p : ℕ) → m + (n + p) ≡ n + (m + p)
+-swap m n p =
  begin
    m + (n + p)
  ≡⟨ sym (+-assoc m n p) ⟩
    (m + n) + p
  ≡⟨ cong (_+ p) (+-comm m n)⟩
    (n + m) + p
  ≡⟨ +-assoc n m p ⟩
    n + (m + p)
  ∎

*-distrib-+ : ∀ (m n p : ℕ) → (m + n) * p ≡ m * p + n * p
*-distrib-+ m zero p =
  begin
    (m + zero) * p
  ≡⟨ cong (_* p) (+-identityʳ m) ⟩
    m * p
  ≡⟨ sym (+-identityʳ (m * p)) ⟩
    (m * p) + zero
  ≡⟨⟩
    (m * p) + zero * p 
  ∎

*-distrib-+ m (suc n) p = 
  begin
    (m + suc n) * p
  ≡⟨ cong (_* p) (+-suc m n) ⟩
    (suc (m + n)) * p
  ≡⟨⟩
    p + (m + n) * p
  ≡⟨ cong (p +_) (*-distrib-+ m n p)⟩
    p + (m * p + n * p)
  ≡⟨ +-swap p (m * p) (n * p)⟩
    m * p + (p + n * p)
  ≡⟨⟩
    m * p + (suc n) * p
  ∎

*-assoc : ∀ (m n p : ℕ) → (m * n) * p ≡ m * (n * p)
*-assoc m n p =
  begin
    m n p
  ∎